added Word

Lib/Word.v
@@ -7,15 +7,13 @@ Definition minimize_eq_proof{A: Type}(eq_dec: forall (x y: A), {x = y} + {x <> y
   | right n => match n pf: False with end
   end.
 
-Notation pow2 := (Z.pow 2).
-
 Section Word.
   Section fixedWidth.
     Variable width : nat.
 
     Declare Scope word_scope.
 
-    Local Notation wrap_value n := (Z.modulo n (pow2 (Z.of_nat width))).
+    Local Notation wrap_value n := (Z.modulo n (Z.pow 2 (Z.of_nat width))).
 
     (* Word is a record with two fields wordVal and wordBound *)
     Record word := mk {wordVal : Z ;
@@ -43,7 +41,7 @@ Section Word.
     
     Definition wordToNat (w : word) := Z.to_nat (wordVal w).
 
-    Definition wmax := ZToWord ((2 ^ (Z.of_nat width))%Z - 1).
+    Definition wones := ZToWord ((2 ^ (Z.of_nat width))%Z - 1).
       
     Definition wadd x y := ZToWord (Z.add (wordVal x) (wordVal y)).
 
@@ -55,11 +53,11 @@ Section Word.
 
     Definition wxor x y := ZToWord (Z.lxor (wordVal x) (wordVal y)).
 
-    Definition wneg x := ZToWord (Z.sub (pow2 (Z.of_nat width)) (wordVal x)).
+    Definition wneg x := ZToWord (Z.sub (Z.pow 2 (Z.of_nat width)) (wordVal x)).
 
     Definition wnot x := ZToWord (Z.sub (wordVal (wneg x)) 1).
 
-    Definition wuand x := Z.eqb (wordVal wmax) (wordVal x).
+    Definition wuand x := Z.eqb (wordVal wones) (wordVal x).
 
     Definition wuor x := negb (Z.eqb (wordVal (ZToWord 0)) (wordVal x)).
 
@@ -85,9 +83,9 @@ Section Word.
 
     Definition wmod x y := ZToWord (Z.modulo (wordVal x) (wordVal y)).
 
-    Definition wslu x y := ZToWord (Z.mul (wordVal x) (pow2 (wordVal y))).
+    Definition wslu x y := ZToWord (Z.mul (wordVal x) (Z.pow 2 (wordVal y))).
 
-    Definition wsru x y := ZToWord (Z.div (wordVal x) (pow2 (wordVal y))).
+    Definition wsru x y := ZToWord (Z.div (wordVal x) (Z.pow 2 (wordVal y))).
 
     Definition weqb x y := Z.eqb (wordVal x) (wordVal y).
 
@@ -99,11 +97,11 @@ Section Word.
     ZToWord lsb (wordVal outSz w).
 
   Definition truncMsb {msb outSz} (w : @word outSz) : @word msb :=
-    ZToWord msb (Z.div (wordVal outSz w) (pow2 (Z.of_nat (Nat.sub outSz msb)))).
+    ZToWord msb (Z.div (wordVal outSz w) (Z.pow 2 (Z.of_nat (Nat.sub outSz msb)))).
 
 
   Definition wconcat {msb lsb outSz} (w1 : @word msb) (w2 : @word lsb) :  @word outSz :=
-    ZToWord outSz (Z.add (Z.mul (wordVal msb w1) (pow2 (Z.of_nat lsb))) (wordVal lsb w2)).
+    ZToWord outSz (Z.add (Z.mul (wordVal msb w1) (Z.pow 2 (Z.of_nat lsb))) (wordVal lsb w2)).
 
   Definition get_msb {sz} (w : @word sz) : @word 1 :=
     (@truncMsb 1 sz w).
@@ -112,13 +110,13 @@ Section Word.
     (@truncLsb 1 sz w).
 
   Definition wnon_neg {sz} (w : @word sz) : bool :=
-    (Z.ltb (wordVal _ w) (pow2 (Z.of_nat (sz - 1)))).
+    (Z.ltb (wordVal _ w) (Z.pow 2 (Z.of_nat (sz - 1)))).
   
   Definition twosComplement {sz} (w: @word sz) : @word sz :=
-    ZToWord _ (Z.sub (pow2 (Z.of_nat sz)) (wordVal _ w)).
+    ZToWord _ (Z.sub (Z.pow 2 (Z.of_nat sz)) (wordVal _ w)).
 
   Definition wordToSignedZ {sz} (w: @word sz) : Z :=
-    if Z.ltb (wordVal _ w) (pow2 (Z.of_nat (sz - 1)))
+    if Z.ltb (wordVal _ w) (Z.pow 2 (Z.of_nat (sz - 1)))
     then wordVal _ w
     else Z.opp (wordVal _ (twosComplement w)).
 
@@ -137,17 +135,17 @@ Section Word.
   Definition wsra {sz1 sz2: nat} (w1: @word sz1) (w2 : @word sz2) : @word sz1 :=
     @signedZToWord sz1 (Z.div (if wnon_neg w1
                                then wordVal _ w1
-                               else wordToSignedZ w1) (pow2 (wordVal _ w2))).
+                               else wordToSignedZ w1) (Z.pow 2 (wordVal _ w2))).
   
   Definition whd sz (w : word (S sz)) := @truncMsb 1 _ w.
 
   Definition wtail sz (w : word (S sz)) := @truncLsb sz _ w.
 
   Definition wsplitl (sz1 sz2 : nat) (w : @word (sz1 + sz2)) : @word sz1 :=
-    ZToWord _ (wordVal _ w / (pow2 (Z.of_nat sz2)))%Z.
+    ZToWord _ (wordVal _ w / (Z.pow 2 (Z.of_nat sz2)))%Z.
 
   Definition wsplitr (sz1 sz2 : nat) (w : @word (sz1 + sz2)) : @word sz2 :=
-    ZToWord _ ((wordVal _ w) mod (pow2 (Z.of_nat sz2)))%Z.
+    ZToWord _ ((wordVal _ w) mod (Z.pow 2 (Z.of_nat sz2)))%Z.
   
 End Word.
 
@@ -166,8 +164,10 @@ Module Notations.
 
   Notation "WO~0" := (ZToWord 1 0) : word_scope.
   Notation "WO~1" := (ZToWord 1 1) : word_scope.
-  
+
+  Delimit Scope word_scope with word.
 End Notations.
+Notation wzero sz := (ZToWord sz 0).
 
 Export Notations.
 Export ZArith.
