Lib/WordProperties.v
@@ -397,7 +397,7 @@ Proof.
   - apply Z.mod_small; auto.
 Qed.
 
-Lemma Zpow_1_0 : forall b, (pow2 b = 1)%Z -> b = 0%Z.
+Lemma Zpow_1_0 : forall b, (Z.pow 2 b = 1)%Z -> b = 0%Z.
 Proof.
   repeat intro.
   destruct (Z_lt_le_dec 0 b).
@@ -408,7 +408,7 @@ Proof.
 Qed.
 
 
-Lemma wmax_wzero : forall sz, (sz > 0) -> wmax sz <> ZToWord sz 0.
+Lemma wones_wzero : forall sz, (sz > 0) -> wones sz <> ZToWord sz 0.
 Proof.
   repeat intro.
   eapply (f_equal (wordVal _)) in H0.
@@ -423,7 +423,7 @@ Qed.
 
 
 Lemma wordToZ_ZToWord: forall (sz : nat) (w : Z),
-    (0 <= w < pow2 (Z.of_nat sz))%Z -> wordVal _ (ZToWord sz w) = w.
+    (0 <= w < Z.pow 2 (Z.of_nat sz))%Z -> wordVal _ (ZToWord sz w) = w.
 Proof.
   intros.
   arithmetizeWord.
@@ -612,28 +612,26 @@ Proof.
   lia.
 Qed.
 
-Lemma combine_wmax_WO sz:
+Lemma combine_wones_WO sz:
   forall w, w <> ZToWord sz 0 ->
-            @truncMsb 1 (sz+1)
-                      (@wadd _ (@wconcat sz 1 (sz+1) (wmax sz) (ZToWord 1 0))
-                             (@wconcat _ 1 _ w (@ZToWord 1 0)))
-            = @wconcat 1 0 1 (wmax 1) (ZToWord 0 0).
+            truncMsb (outSz := sz+1)
+                     (wadd _ (wconcat (wones sz) (ZToWord 1 0))
+                           (wconcat w (@ZToWord 1 0)))
+            = (WO~1)%word.
 Proof.
   intros.
   arithmetizeWord.
-  rewrite Z.mod_1_l.
-  * rewrite Z.pow_pos_fold.
+  rewrite Z.mod_1_l by reflexivity.
+  + rewrite Z.pow_pos_fold.
     simpl in *.
-    rewrite Z.mod_0_l.
+    rewrite Z.mod_0_l by (let H := fresh in intro H; discriminate).
     rewrite Nat.add_sub.
     rewrite Z.pow_pos_fold.
     rewrite Z.pow_1_r.
     repeat (rewrite Z.add_0_r).
+    
+    simpl.
     admit.
-    intro.
-    rewrite Z.pow_pos_fold in H1; try lia.    
-  * rewrite Z.pow_pos_fold.
-    lia.
 Admitted.
 
 Lemma word1_neq (w: word 1):
@@ -686,7 +684,7 @@ Proof.
 Qed.
 
 Lemma truncLsb_fits_ZToWord n sz:
-  (0 <= n < pow2 (Z.of_nat sz))%Z -> 
+  (0 <= n < Z.pow 2 (Z.of_nat sz))%Z -> 
   (@truncLsb sz (sz+1) (ZToWord (sz + 1) n) = ZToWord sz n).
 Proof.
   intro.
